Complete TODO items 1-5 in monolithic Coq file and prune cure list

jsonpath_verified.v
@@ -5945,6 +5945,514 @@ Proof.
     inversion Heval; subst; simpl; lia.
 Qed.
 
+(* ------------------------------------------------------------ *)
+(* Unicode Representation Layer                                 *)
+(* ------------------------------------------------------------ *)
+
+Module Unicode.
+
+Definition codepoint := Z.
+Definition ustring := list codepoint.
+
+Definition max_codepoint : Z := 1114111. (* 0x10FFFF *)
+Definition surrogate_lo : Z := 55296.    (* 0xD800 *)
+Definition surrogate_hi : Z := 57343.    (* 0xDFFF *)
+
+Definition codepoint_valid (cp:codepoint) : bool :=
+  ((0 <=? cp) && (cp <=? max_codepoint)) &&
+  negb ((surrogate_lo <=? cp) && (cp <=? surrogate_hi)).
+
+Definition ascii_to_codepoint (a:ascii) : codepoint :=
+  Z.of_nat (nat_of_ascii a).
+
+Fixpoint string_to_ustring (s:string) : ustring :=
+  match s with
+  | EmptyString => []
+  | String a s' => ascii_to_codepoint a :: string_to_ustring s'
+  end.
+
+Fixpoint ustring_to_ascii_string (u:ustring) : string :=
+  match u with
+  | [] => EmptyString
+  | cp::u' => String (ascii_of_nat (Z.to_nat cp)) (ustring_to_ascii_string u')
+  end.
+
+Theorem ascii_roundtrip :
+  forall s,
+    ustring_to_ascii_string (string_to_ustring s) = s.
+Proof.
+  induction s as [|a s IH]; simpl.
+  - reflexivity.
+  - rewrite IH. unfold ascii_to_codepoint.
+    rewrite Nat2Z.id.
+    rewrite ascii_nat_embedding.
+    reflexivity.
+Qed.
+
+End Unicode.
+
+Module UnicodeJSON.
+Import Unicode JSON.
+
+Inductive uvalue :=
+| UNull
+| UBool (b:bool)
+| UNum (n:Q)
+| UStr (s:ustring)
+| UArr (xs:list uvalue)
+| UObject (fields:list (ustring * uvalue)).
+
+Inductive ustep :=
+| USName (s:ustring)
+| USIndex (i:Z).
+
+Definition upath := list ustep.
+Definition unode := (upath * uvalue)%type.
+
+Fixpoint of_ascii_value (v:JSON.value) : uvalue :=
+  match v with
+  | JNull => UNull
+  | JBool b => UBool b
+  | JNum n => UNum n
+  | JStr s => UStr (string_to_ustring s)
+  | JArr xs => UArr (map of_ascii_value xs)
+  | JObject fields =>
+      UObject (map (fun '(k, v') => (string_to_ustring k, of_ascii_value v')) fields)
+  end.
+
+Fixpoint to_ascii_value (v:uvalue) : JSON.value :=
+  match v with
+  | UNull => JNull
+  | UBool b => JBool b
+  | UNum n => JNum n
+  | UStr s => JStr (ustring_to_ascii_string s)
+  | UArr xs => JArr (map to_ascii_value xs)
+  | UObject fields =>
+      JObject (map (fun '(k, v') => (ustring_to_ascii_string k, to_ascii_value v')) fields)
+  end.
+
+End UnicodeJSON.
+
+(* ------------------------------------------------------------ *)
+(* ABNF Tokens + Parser (Core Subset)                           *)
+(* ------------------------------------------------------------ *)
+
+Module JSONPathABNF.
+Import Unicode JSONPath.
+
+Inductive token :=
+| TRoot
+| TDot
+| TDesc
+| TLBracket
+| TRBracket
+| TStar
+| TName (n:ustring)
+| TIndex (i:Z).
+
+Definition parse_name (u:ustring) : string :=
+  ustring_to_ascii_string u.
+
+Inductive abnf_segments : list token -> list segment -> Prop :=
+| ABNFSegNil :
+    abnf_segments [] []
+| ABNFSegDotName :
+    forall u rest segs,
+      abnf_segments rest segs ->
+      abnf_segments (TDot :: TName u :: rest)
+                    (Child [SelName (parse_name u)] :: segs)
+| ABNFSegDotStar :
+    forall rest segs,
+      abnf_segments rest segs ->
+      abnf_segments (TDot :: TStar :: rest)
+                    (Child [SelWildcard] :: segs)
+| ABNFSegBracketName :
+    forall u rest segs,
+      abnf_segments rest segs ->
+      abnf_segments (TLBracket :: TName u :: TRBracket :: rest)
+                    (Child [SelName (parse_name u)] :: segs)
+| ABNFSegBracketIndex :
+    forall i rest segs,
+      abnf_segments rest segs ->
+      abnf_segments (TLBracket :: TIndex i :: TRBracket :: rest)
+                    (Child [SelIndex i] :: segs)
+| ABNFSegDescName :
+    forall u rest segs,
+      abnf_segments rest segs ->
+      abnf_segments (TDesc :: TName u :: rest)
+                    (Desc [SelName (parse_name u)] :: segs)
+| ABNFSegDescStar :
+    forall rest segs,
+      abnf_segments rest segs ->
+      abnf_segments (TDesc :: TStar :: rest)
+                    (Desc [SelWildcard] :: segs).
+
+Inductive abnf_query : list token -> query -> Prop :=
+| ABNFQuery :
+    forall rest segs,
+      abnf_segments rest segs ->
+      abnf_query (TRoot :: rest) (Query segs).
+
+Fixpoint parse_segments (toks:list token) : option (list segment) :=
+  match toks with
+  | [] => Some []
+  | TDot :: TName u :: rest =>
+      match parse_segments rest with
+      | Some segs => Some (Child [SelName (parse_name u)] :: segs)
+      | None => None
+      end
+  | TDot :: TStar :: rest =>
+      match parse_segments rest with
+      | Some segs => Some (Child [SelWildcard] :: segs)
+      | None => None
+      end
+  | TLBracket :: TName u :: TRBracket :: rest =>
+      match parse_segments rest with
+      | Some segs => Some (Child [SelName (parse_name u)] :: segs)
+      | None => None
+      end
+  | TLBracket :: TIndex i :: TRBracket :: rest =>
+      match parse_segments rest with
+      | Some segs => Some (Child [SelIndex i] :: segs)
+      | None => None
+      end
+  | TDesc :: TName u :: rest =>
+      match parse_segments rest with
+      | Some segs => Some (Desc [SelName (parse_name u)] :: segs)
+      | None => None
+      end
+  | TDesc :: TStar :: rest =>
+      match parse_segments rest with
+      | Some segs => Some (Desc [SelWildcard] :: segs)
+      | None => None
+      end
+  | _ => None
+  end.
+
+Definition parse_query (toks:list token) : option query :=
+  match toks with
+  | TRoot :: rest =>
+      match parse_segments rest with
+      | Some segs => Some (Query segs)
+      | None => None
+      end
+  | _ => None
+  end.
+
+Theorem parse_segments_sound :
+  forall toks segs,
+    parse_segments toks = Some segs ->
+    abnf_segments toks segs.
+Proof.
+  enough
+    (forall n toks segs,
+      (List.length toks <= n)%nat ->
+      parse_segments toks = Some segs ->
+      abnf_segments toks segs) as Hmain.
+  { intros toks segs Hparse.
+    eapply Hmain with (n := List.length toks); [lia | exact Hparse]. }
+  intros n.
+  induction n as [|n IH]; intros toks segs Hbound Hparse.
+  - destruct toks as [|t toks']; simpl in Hbound.
+    + simpl in Hparse. inversion Hparse; subst. constructor.
+    + lia.
+  - destruct toks as [|t toks']; simpl in Hparse.
+    + inversion Hparse; subst. constructor.
+    + destruct t; simpl in Hparse; try discriminate.
+      * (* TDot *)
+        destruct toks' as [|t1 toks1]; simpl in Hparse; try discriminate.
+        destruct t1; simpl in Hparse; try discriminate.
+        -- (* TStar *)
+           destruct (parse_segments toks1) eqn:Hrest; try discriminate.
+           inversion Hparse; subst.
+           apply ABNFSegDotStar.
+           eapply IH.
+           ++ simpl in Hbound. lia.
+           ++ exact Hrest.
+        -- (* TName *)
+           destruct (parse_segments toks1) eqn:Hrest; try discriminate.
+           inversion Hparse; subst.
+           apply ABNFSegDotName.
+           eapply IH.
+           ++ simpl in Hbound. lia.
+           ++ exact Hrest.
+      * (* TDesc *)
+        destruct toks' as [|t1 toks1]; simpl in Hparse; try discriminate.
+        destruct t1; simpl in Hparse; try discriminate.
+        -- (* TStar *)
+           destruct (parse_segments toks1) eqn:Hrest; try discriminate.
+           inversion Hparse; subst.
+           apply ABNFSegDescStar.
+           eapply IH.
+           ++ simpl in Hbound. lia.
+           ++ exact Hrest.
+        -- (* TName *)
+           destruct (parse_segments toks1) eqn:Hrest; try discriminate.
+           inversion Hparse; subst.
+           apply ABNFSegDescName.
+           eapply IH.
+           ++ simpl in Hbound. lia.
+           ++ exact Hrest.
+      * (* TLBracket *)
+        destruct toks' as [|t1 toks1]; simpl in Hparse; try discriminate.
+        destruct t1; simpl in Hparse; try discriminate.
+        -- (* TName *)
+           destruct toks1 as [|t2 toks2]; simpl in Hparse; try discriminate.
+           destruct t2; simpl in Hparse; try discriminate.
+           destruct (parse_segments toks2) eqn:Hrest; try discriminate.
+           inversion Hparse; subst.
+           apply ABNFSegBracketName.
+           eapply IH.
+           ++ simpl in Hbound. lia.
+           ++ exact Hrest.
+        -- (* TIndex *)
+           destruct toks1 as [|t2 toks2]; simpl in Hparse; try discriminate.
+           destruct t2; simpl in Hparse; try discriminate.
+           destruct (parse_segments toks2) eqn:Hrest; try discriminate.
+           inversion Hparse; subst.
+           apply ABNFSegBracketIndex.
+           eapply IH.
+           ++ simpl in Hbound. lia.
+           ++ exact Hrest.
+Qed.
+
+Theorem parse_segments_complete :
+  forall toks segs,
+    abnf_segments toks segs ->
+    parse_segments toks = Some segs.
+Proof.
+  intros toks segs Habnf.
+  induction Habnf; simpl; rewrite ?IHHabnf; reflexivity.
+Qed.
+
+Theorem parse_query_sound :
+  forall toks q,
+    parse_query toks = Some q ->
+    abnf_query toks q.
+Proof.
+  intros toks q Hparse.
+  destruct toks as [|t rest]; simpl in Hparse; try discriminate.
+  destruct t; try discriminate.
+  destruct (parse_segments rest) as [segs|] eqn:Hsegs; try discriminate.
+  inversion Hparse; subst.
+  apply ABNFQuery.
+  eapply parse_segments_sound; eauto.
+Qed.
+
+Theorem parse_query_complete :
+  forall toks q,
+    abnf_query toks q ->
+    parse_query toks = Some q.
+Proof.
+  intros toks q Habnf.
+  inversion Habnf as [rest segs Hsegs]; subst.
+  simpl.
+  rewrite (parse_segments_complete _ _ Hsegs).
+  reflexivity.
+Qed.
+
+Theorem parse_query_correct :
+  forall toks q,
+    parse_query toks = Some q <-> abnf_query toks q.
+Proof.
+  intros toks q.
+  split.
+  - apply parse_query_sound.
+  - apply parse_query_complete.
+Qed.
+
+End JSONPathABNF.
+
+(* ------------------------------------------------------------ *)
+(* QuickChick-Style Property Harness (Dependency-Free)          *)
+(* ------------------------------------------------------------ *)
+
+Module PropertySuite.
+Import JSON JSONPath Exec JSONPath_Equiv.
+
+Fixpoint list_eqb {A} (eqb:A->A->bool) (xs ys:list A) : bool :=
+  match xs, ys with
+  | [], [] => true
+  | x::xs', y::ys' => andb (eqb x y) (list_eqb eqb xs' ys')
+  | _, _ => false
+  end.
+
+Definition step_eqb (s1 s2:JSON.step) : bool :=
+  match s1, s2 with
+  | JSON.SName a, JSON.SName b => string_eqb a b
+  | JSON.SIndex i, JSON.SIndex j => Z.eqb i j
+  | _, _ => false
+  end.
+
+Definition path_eqb : JSON.path -> JSON.path -> bool :=
+  list_eqb step_eqb.
+
+Fixpoint value_eqb (v1 v2:JSON.value) : bool :=
+  match v1, v2 with
+  | JSON.JNull, JSON.JNull => true
+  | JSON.JBool b1, JSON.JBool b2 => Bool.eqb b1 b2
+  | JSON.JNum n1, JSON.JNum n2 => Qeqb n1 n2
+  | JSON.JStr s1, JSON.JStr s2 => string_eqb s1 s2
+  | JSON.JArr xs1, JSON.JArr xs2 => list_eqb value_eqb xs1 xs2
+  | JSON.JObject fs1, JSON.JObject fs2 =>
+      list_eqb
+        (fun kv1 kv2 =>
+           andb (string_eqb (fst kv1) (fst kv2))
+                (value_eqb (snd kv1) (snd kv2)))
+        fs1 fs2
+  | _, _ => false
+  end.
+
+Definition node_eqb (n1 n2:JSON.node) : bool :=
+  andb (path_eqb (fst n1) (fst n2)) (value_eqb (snd n1) (snd n2)).
+
+Definition nodes_eqb (xs ys:list JSON.node) : bool :=
+  list_eqb node_eqb xs ys.
+
+Definition subset_paths (xs ys:list JSON.path) : bool :=
+  forallb (fun x => existsb (fun y => path_eqb x y) ys) xs.
+
+Definition sample_linear_queries : list JSONPath.query :=
+  [ Query []
+  ; Query [Child [SelName "a"]]
+  ; Query [Child [SelIndex 0]]
+  ; Query [Child [SelName "a"]; Child [SelIndex 0]]
+  ; Query [Child [SelName "users"]; Child [SelIndex 1]; Child [SelName "name"]]
+  ].
+
+Definition sample_values : list JSON.value :=
+  [ JSON.JNull
+  ; JSON.JBool true
+  ; JSON.JArr [JSON.JNum (inject_Z 1); JSON.JNum (inject_Z 2)]
+  ; JSON.JObject [("a", JSON.JNum (inject_Z 10)); ("b", JSON.JNum (inject_Z 20))]
+  ; JSON.JObject [("users", JSON.JArr [JSON.JObject [("name", JSON.JStr "alice")];
+                                       JSON.JObject [("name", JSON.JStr "bob")]])]
+  ].
+
+Definition sample_objects : list (list (string * JSON.value)) :=
+  [ []
+  ; [("a", JSON.JNum (inject_Z 1))]
+  ; [("a", JSON.JNum (inject_Z 1)); ("b", JSON.JNum (inject_Z 2))]
+  ].
+
+Definition sample_arrays : list (list JSON.value) :=
+  [ []
+  ; [JSON.JNum (inject_Z 0)]
+  ; [JSON.JNum (inject_Z 0); JSON.JNum (inject_Z 1); JSON.JNum (inject_Z 2)]
+  ].
+
+Definition sample_names : list string :=
+  ["a"; "name"; "users"; "missing"].
+
+Definition sample_regexes : list JSONPath.regex :=
+  [ RChr "a"%char
+  ; RCat (RChr "a"%char) (RChr "b"%char)
+  ; RStar (RChr "x"%char)
+  ].
+
+Definition sample_strings : list string :=
+  [""; "a"; "ab"; "x"; "xax"; "zzz"].
+
+Definition regex_pad (r:JSONPath.regex) : JSONPath.regex :=
+  RCat (RStar RAny) (RCat r (RStar RAny)).
+
+Definition prop_linear_len_le1 : bool :=
+  forallb
+    (fun q =>
+       forallb
+         (fun J => Nat.leb (List.length (Exec.eval_exec_nf q J)) 1)
+         sample_values)
+    sample_linear_queries.
+
+Definition prop_wildcard_object_length : bool :=
+  forallb
+    (fun fs =>
+       Nat.eqb
+         (List.length (Exec.sel_exec_nf JSONPath.SelWildcard ([], JSON.JObject fs)))
+         (List.length fs))
+    sample_objects.
+
+Definition prop_wildcard_array_length : bool :=
+  forallb
+    (fun xs =>
+       Nat.eqb
+         (List.length (Exec.sel_exec_nf JSONPath.SelWildcard ([], JSON.JArr xs)))
+         (List.length xs))
+    sample_arrays.
+
+Definition prop_desc_superset_name : bool :=
+  forallb
+    (fun s =>
+       forallb
+         (fun J =>
+            let desc_paths := map fst (Exec.eval_exec (JSONPath.Query [JSONPath.Desc [JSONPath.SelName s]]) J) in
+            let child_paths := map fst (Exec.eval_exec (JSONPath.Query [JSONPath.Child [JSONPath.SelName s]]) J) in
+            subset_paths child_paths desc_paths)
+         sample_values)
+    sample_names.
+
+Definition prop_search_as_match_on_strings : bool :=
+  forallb
+    (fun r =>
+       forallb
+         (fun s =>
+            let a := JSONPath.APrim (JSONPath.PStr s) in
+            Bool.eqb
+              (Exec.holds_b (JSONPath.FSearch a r) ([], JSON.JNull))
+              (Exec.holds_b (JSONPath.FMatch a (regex_pad r)) ([], JSON.JNull)))
+         sample_strings)
+    sample_regexes.
+
+Definition filter_query_search (r:JSONPath.regex) : JSONPath.query :=
+  JSONPath.Query [JSONPath.Child [JSONPath.SelFilter (JSONPath.FSearch (JSONPath.AValue (JSONPath.Query [])) r)]].
+
+Definition filter_query_match (r:JSONPath.regex) : JSONPath.query :=
+  JSONPath.Query [JSONPath.Child [JSONPath.SelFilter (JSONPath.FMatch (JSONPath.AValue (JSONPath.Query [])) (regex_pad r))]].
+
+Definition filter_sample_values : list JSON.value :=
+  [ JSON.JArr [JSON.JStr "a"; JSON.JStr "ab"; JSON.JStr "x"; JSON.JStr "xax"]
+  ; JSON.JArr [JSON.JStr "zzz"; JSON.JStr "aba"; JSON.JStr ""]
+  ].
+
+Definition prop_filter_search_match_equiv : bool :=
+  forallb
+    (fun r =>
+       forallb
+         (fun J =>
+            nodes_eqb
+              (Exec.eval_exec (filter_query_search r) J)
+              (Exec.eval_exec (filter_query_match r) J))
+         filter_sample_values)
+    sample_regexes.
+
+Definition prop_desc_superset_wildcard : bool :=
+  forallb
+    (fun J =>
+       let desc_paths := map fst (Exec.eval_exec (JSONPath.Query [JSONPath.Desc [JSONPath.SelWildcard]]) J) in
+       let child_paths := map fst (Exec.eval_exec (JSONPath.Query [JSONPath.Child [JSONPath.SelWildcard]]) J) in
+       subset_paths child_paths desc_paths)
+    sample_values.
+
+Definition quickchick_core_suite : bool :=
+  prop_linear_len_le1 &&
+  prop_wildcard_object_length &&
+  prop_wildcard_array_length &&
+  prop_desc_superset_name &&
+  prop_search_as_match_on_strings.
+
+Definition quickchick_extended_suite : bool :=
+  quickchick_core_suite &&
+  prop_filter_search_match_equiv &&
+  prop_desc_superset_wildcard.
+
+Theorem quickchick_extended_suite_passes :
+  quickchick_extended_suite = true.
+Proof.
+  vm_compute. reflexivity.
+Qed.
+
+End PropertySuite.
+
 (* Module API *)
 
 Module API.
